theories/examples/enclaves/trusted_memory_readout_main_spec.v
@@ -1,0 +1,476 @@
+From iris.proofmode Require Import proofmode.
+From cap_machine Require Import rules logrel fundamental.
+From cap_machine Require Import proofmode.
+From cap_machine Require Import assert macros_new.
+From cap_machine Require Import
+  trusted_memory_readout_code
+.
+
+Section trusted_memory_readout_main.
+  Context {Σ:gFunctors} {ceriseg:ceriseG Σ} {sealsg: sealStoreG Σ}
+          {nainv: logrel_na_invs Σ}
+          {reservedaddresses : ReservedAddresses}
+          `{MP: MachineParameters}.
+  Context {CS: ClientSensor}.
+
+  (* ---------------------------------- *)
+  (* ----- TRUSTED READOUT *MAIN* ----- *)
+  (* ---------------------------------- *)
+
+  (* Expect:
+     - PC := (RWX, main, main_end, main)
+     - R0 := (RWX, adv, adv_end, adv)
+   *)
+
+  (** Specification init code *)
+  Lemma trusted_memory_readout_main_init_spec
+    (b_main : Addr)
+    (pc_v : Version)
+    (assert_lt_offset : Z)
+    (w1 wadv : LWord)
+    φ :
+
+    let e_main := (b_main ^+ trusted_memory_readout_main_len)%a in
+    let a_callback := (b_main ^+ trusted_memory_readout_main_init_len)%a in
+    let a_data := (b_main ^+ trusted_memory_readout_main_code_len)%a in
+
+    let trusted_memory_readout_main := trusted_memory_readout_main_code assert_lt_offset in
+    ContiguousRegion b_main trusted_memory_readout_main_len ->
+    ⊢ ((
+          codefrag b_main pc_v trusted_memory_readout_main
+
+          ∗ PC ↦ᵣ LCap RWX b_main e_main b_main pc_v
+          ∗ r_t0 ↦ᵣ wadv
+          ∗ r_t1 ↦ᵣ w1
+          (* NOTE this post-condition stops after jumping to the adversary *)
+          ∗ ▷ ( codefrag b_main pc_v trusted_memory_readout_main
+                ∗ PC ↦ᵣ updatePcPermL wadv
+                ∗ r_t0 ↦ᵣ wadv
+                ∗ r_t1 ↦ᵣ (LCap E b_main e_main a_callback pc_v)
+                  -∗ WP Seq (Instr Executable) {{ φ }}))
+         -∗ WP Seq (Instr Executable) {{ φ }})%I.
+  Proof.
+
+    (* We define a local version of solve_addr, which subst and unfold every computed addresses  *)
+    Local Tactic Notation "solve_addr'" :=
+      repeat (lazymatch goal with x := _ |- _ => subst x end)
+      ; repeat (match goal with
+                  | H: ContiguousRegion _ _  |- _ =>
+                      rewrite /ContiguousRegion /trusted_memory_readout_main_len in H
+                end)
+      ; rewrite !/trusted_memory_readout_main_code_len /trusted_memory_readout_main_len
+          /trusted_memory_readout_main_init_len /trusted_memory_readout_main_callback_len
+      ; solve_addr.
+
+    intros ???? Hregion.
+    iIntros "(Hcode & HPC & Hr0 & Hr1 & Hφ)".
+    codefrag_facts "Hcode".
+    iGo "Hcode".
+    rewrite decode_encode_perm_inv; by cbn.
+    rewrite decode_encode_perm_inv.
+    iGo "Hcode".
+    iApply "Hφ".
+    iFrame.
+  Qed.
+
+  (** Specification callback code *)
+
+  (* Define all the invariants *)
+  (* Linking table invariant *)
+  Definition link_table_inv
+    v_link
+    assert_entry b_assert e_assert v_assert link_tableN :=
+    na_inv logrel_nais link_tableN
+         ((assert_entry, v_link) ↦ₐ LCap E b_assert e_assert b_assert v_assert)%I.
+
+  (* Assert invariants *)
+  Definition assert_inv b_a a_flag e_a v_assert assertN :=
+    na_inv logrel_nais assertN (assert_inv b_a a_flag e_a v_assert).
+  Definition flag_inv a_flag v_flag flag_assertN :=
+    inv flag_assertN ((a_flag,v_flag) ↦ₐ LInt 0%Z).
+
+
+  Lemma trusted_memory_readout_callback_code_spec
+    (E : coPset) (assertN flag_assertN link_tableN : namespace)
+    (b_main pc_b pc_e : Addr)
+    (pc_v : Version)
+
+    (b_link a_link e_link assert_entry : Addr) (* linking *)
+    (assert_lt_offset : Z)
+    (b_assert e_assert a_flag : Addr) (v_assert : Version) (* assert *)
+    (w0 w1 w2 w3 w4 w5 : LWord)
+    φ :
+
+    let v_link := pc_v in
+    let link_cap := LCap RO b_link e_link a_link v_link in
+
+    let e_main := (b_main ^+ trusted_memory_readout_main_len)%a in
+    let a_callback := (b_main ^+ trusted_memory_readout_main_init_len)%a in
+    let a_data := (b_main ^+ trusted_memory_readout_main_code_len)%a in
+
+    let trusted_memory_readout_main := trusted_memory_readout_main_code assert_lt_offset in
+    ContiguousRegion b_main trusted_memory_readout_main_len ->
+
+    ↑link_tableN ⊆ E ->
+    ↑assertN ⊆ E ->
+    ↑clientN ⊆ E ->
+    ↑sensorN ⊆ E ->
+    assertN ## link_tableN ->
+
+    (a_link + assert_lt_offset)%a = Some assert_entry →
+    withinBounds b_link e_link assert_entry = true ->
+    SubBounds pc_b pc_e b_main e_main ->
+
+    (link_table_inv
+       v_link
+       assert_entry b_assert e_assert v_assert link_tableN
+    ∗ assert_inv b_assert a_flag e_assert v_assert assertN
+    ∗ flag_inv a_flag v_assert flag_assertN)
+    ∗ system_inv (enclaves_map := contract_ts_enclaves_map)
+    ∗ interp w1
+    ∗ interp w0
+
+    ⊢ (( codefrag b_main pc_v trusted_memory_readout_main
+          ∗ ((a_data)%a, pc_v) ↦ₐ link_cap
+          ∗ ((a_data ^+ 1)%a, pc_v) ↦ₐ (LCap RWX b_main e_main a_data pc_v)
+          ∗ PC ↦ᵣ LCap RX pc_b pc_e a_callback pc_v
+          ∗ r_t0 ↦ᵣ w0
+          ∗ r_t1 ↦ᵣ w1
+          ∗ r_t2 ↦ᵣ w2
+          ∗ r_t3 ↦ᵣ w3
+          ∗ r_t4 ↦ᵣ w4
+          ∗ r_t5 ↦ᵣ w5
+          ∗ na_own logrel_nais E
+
+          ∗ ▷ ( codefrag b_main pc_v trusted_memory_readout_main
+                ∗ ((a_data)%a, pc_v) ↦ₐ link_cap
+                ∗ ((a_data ^+ 1)%a, pc_v) ↦ₐ (LCap RWX b_main e_main a_data pc_v)
+
+                ∗ PC ↦ᵣ LCap RX pc_b pc_e (a_data ^+ (-2))%a pc_v
+                ∗ r_t0 ↦ᵣ LInt 0
+                ∗ r_t1 ↦ᵣ LInt 0
+                ∗ r_t2 ↦ᵣ LInt 0
+                ∗ r_t3 ↦ᵣ LInt 0
+                ∗ r_t4 ↦ᵣ LInt 0
+                ∗ r_t5 ↦ᵣ LInt 0
+                ∗ na_own logrel_nais E
+
+                  -∗ WP (Instr Halted) {{ φ }}))
+         -∗ WP Seq (Instr Executable) {{ λ v, φ v ∨ ⌜v = FailedV⌝ }})%I.
+  Proof.
+
+    (* We define a local version of solve_addr, which subst and unfold every computed addresses  *)
+    Local Tactic Notation "solve_addr'" :=
+      repeat (lazymatch goal with x := _ |- _ => subst x end)
+      ; repeat (match goal with
+                  | H: ContiguousRegion _ _  |- _ =>
+                      rewrite /ContiguousRegion /trusted_memory_readout_main_len in H
+                end)
+      ; rewrite !/trusted_memory_readout_main_code_len /trusted_memory_readout_main_len
+          /trusted_memory_readout_main_init_len /trusted_memory_readout_main_callback_len
+      ; solve_addr.
+
+    intros ?????? Hregion HE1 HE2 HE3 HE4 HE_disj Hassert Hlink Hpcbounds.
+
+    iIntros "#[ [HlinkInv [HassertInv HflagInv] ] [ Hcemap_inv [ Hinterp_w1 Hinterp_w0]] ]
+             (Hcode & Hlink_cap & Hdata1 & HPC & Hr0 & Hr1 & Hr2 & Hr3 & Hr4 & Hr5 & Hna & Hcont)".
+    codefrag_facts "Hcode".
+
+    iInstr "Hcode". (* Mov *)
+    iInstr "Hcode". (* Lea *)
+
+    destruct (is_sealedL w0) eqn:Hsealed_w0 ; cycle 1.
+    { (* w0 is not a sealed  *)
+      destruct_lword (w0) ; cbn in Hsealed_w0 ; try done.
+      all: iInstr "Hcode". (* GetOType *)
+      all: iInstr "Hcode". (* Sub *)
+      all: replace (-1 - -1) with 0 by lia.
+      all: iInstr "Hcode". (* Mov *)
+      all: iInstr "Hcode". (* Lea *)
+      all: iInstr "Hcode". (* Jnz *)
+      all: iInstr "Hcode". (* Jmp *)
+      all: iInstr "Hcode". (* Fail *)
+      all: by (wp_end; iRight).
+    }
+
+    destruct w0 as [ ? | ? | o sw0 ]
+    ; cbn in Hsealed_w0 ; try done; clear Hsealed_w0.
+
+    iInstr "Hcode". (* GetOType *)
+    iInstr "Hcode". (* Sub *)
+    replace (o - -1) with (o + 1) by lia.
+    assert (Ho : LInt (o + 1) ≠ LInt 0) by (clear ; intro ; inversion H ; solve_finz).
+    iInstr "Hcode". (* Mov *)
+    iInstr "Hcode". (* Lea *)
+    iInstr "Hcode". (* Jnz *)
+
+    (* Attestation *)
+    iInstr_lookup "Hcode" as "Hi" "Hcode".
+    wp_instr.
+    iMod (inv_acc with "Hcemap_inv") as "(Hcemap & Hclose)"; first solve_ndisj.
+    iDestruct "Hcemap" as (ECn OTn) "(>HEC & ECn_OTn & Hallocated_seals & Hfree_seals & #Hcemap)".
+
+    iApply (wp_estoreid_success_unknown_ec with "[HPC Hr3 Hr2 Hi $HEC]"); try iFrame; try solve_pure.
+    iNext.
+    iIntros (retv) "H".
+    iDestruct "H" as "(Hi & Hr2 & HEC & [(-> & HPC & H)|(-> & HPC & Hr3)])".
+    1: iDestruct "H" as (I tid) "(Hr3 & #Htc_env & [%Hseal %Htidx])".
+    all: iMod ("Hclose" with "[HEC ECn_OTn Hallocated_seals Hfree_seals Hcemap]") as "_"
+    ; [ iExists ECn, OTn; iFrame "HEC Hcemap ECn_OTn Hallocated_seals Hfree_seals"; eauto | iModIntro].
+    all: wp_pure; iInstr_close "Hcode".
+    2:{ wp_end; by iRight. }
+
+    iInstr "Hcode". (* Sub *)
+    destruct (decide (I = hash_client)) as [-> | HnI]
+    ; cycle 1.
+    { (* Not the right enclave *)
+      iInstr "Hcode". (* Jnz *)
+      by (injection; intro Hcontra; lia).
+      iInstr "Hcode". (* Fail *)
+      wp_end; by iRight.
+    }
+    replace ( _ - _) with 0 by lia.
+    iInstr "Hcode". (* Jnz *)
+    iDestruct (interp_valid_sealed with "Hinterp_w0") as (Φ) "Hseal_valid".
+    rewrite /system_inv.
+
+    (* UnSeal *)
+    wp_instr.
+    iInstr_lookup "Hcode" as "Hi" "Hcode".
+    iDestruct (map_of_regs_3 with "HPC Hr1 Hr0") as "[Hmap _]".
+    iApply (wp_UnSeal with "[$Hmap Hi]"); eauto; simplify_map_eq; eauto;
+    try solve_pure.
+    by unfold regs_of; rewrite !dom_insert; set_solver+.
+    iNext. iIntros (regs' retv) "(#Hspec & Hpc_a & Hmap)". iDestruct "Hspec" as %Hspec.
+    destruct Hspec as [ ? ? ? ? ? ? ? Hps Hbounds Hregs'|]; cycle 1.
+    { by wp_pure; wp_end; iRight. }
+
+    incrementLPC_inv as (p''&b_main'&e_main'&a_main'&pc_v'& ? & HPC & Z & Hregs'); simplify_map_eq.
+    repeat (rewrite insert_commute //= insert_insert).
+    replace x with (b_main ^+ 16)%a by solve_addr.
+    clear Z.
+    iDestruct (regs_of_map_3 with "[$Hmap]") as "[HPC [Hr1 Hr0] ]"; eauto; iFrame.
+    wp_pure; iInstr_close "Hcode".
+
+    iAssert (
+        if Z.even a
+        then seal_pred a (Penc client_enclave_pred)
+             ∗ seal_pred (a ^+ 1)%f (Psign client_enclave_pred)
+        else seal_pred (a ^+ -1)%f (Penc client_enclave_pred)
+             ∗ seal_pred a (Psign client_enclave_pred)
+      )%I as "Hts".
+    {
+      iApply "Hcemap"; iFrame "%#∗".
+      iPureIntro.
+      rewrite /ts_enclaves_map lookup_insert_ne //;
+        auto using hash_client_sensor.
+      by simplify_map_eq.
+    }
+
+    destruct (Z.even (finz.to_z a)) eqn:HEven_a
+    ; iDestruct "Hts" as "[Hts_Penc Hts_Psign]"
+    ; iEval (cbn) in "Hts_Penc"
+    ; iEval (cbn) in "Hts_Psign".
+    {
+      iDestruct (seal_pred_valid_sealed_eq with "[$Hts_Penc] Hseal_valid") as "Heqv".
+      iAssert (▷ False)%I as ">%Hcontra"; last done.
+      iDestruct "Hseal_valid" as (sb') "(%Heq & _ & _ & HΦ)".
+      inversion Heq; subst.
+      iSpecialize ("Heqv" $! (LWSealable sb')).
+      iNext.
+      by iRewrite "Heqv".
+    }
+
+    iDestruct (seal_pred_valid_sealed_eq with "[$Hts_Psign] Hseal_valid") as "Heqv".
+    iAssert (▷ sealed_client (LWSealable sb))%I as
+      (use_b use_e use_a use_v) "(>%Hseal_use & Hcontract_use)".
+    { iDestruct "Hseal_valid" as (sb') "(%Heq & _ & _ & HΦ)".
+      inversion Heq; subst.
+      iSpecialize ("Heqv" $! (LWSealable sb')).
+      iNext.
+      iRewrite "Heqv".
+      iFrame "HΦ". }
+    destruct sb ; simplify_eq.
+    iClear "Heqv Hts_Penc Hcemap Hcemap_inv".
+
+    (* Setup callback and jump to client enclave *)
+    iInstr "Hcode". (* Mov *)
+    iInstr "Hcode". (* Lea *)
+    iInstr "Hcode". (* Jmp *)
+
+    iApply ("Hcontract_use" with "[%//] [%//]").
+    iFrame "Hna HPC Hr0".
+    iSplitR. admit.
+    iSplitL "Hr1". iExists _. iExact "Hr1".
+    iSplitL "Hr2". iExists _. iExact "Hr2".
+    iSplitL "Hr3". iExists _. iExact "Hr3".
+    iSplitL "Hr4". iExists _. iExact "Hr4".
+    clear w3 w4.
+    iIntros "!> (Hna & HPC & Hr0 & [%mmio_a Hr1] & Hr2 & (%w3 & Hr3 & Hinterp_w3) & (%w4 & Hr4 & Hinterp_w4))".
+    cbn [updatePcPermL].
+
+    iInstr "Hcode". (* Mov *)
+    iInstr "Hcode". (* Mov *)
+    iInstr "Hcode". (* Mov *)
+    iInstr "Hcode". (* Lea *)
+    iInstr "Hcode". (* Load *)
+
+    subst trusted_memory_readout_main.
+    rewrite /trusted_memory_readout_main_code /trusted_memory_readout_main_code_callback0.
+    subst a_callback.
+    rewrite /trusted_memory_readout_main_init_len.
+
+    subst e_main.
+    focus_block 2%nat "Hcode" as addr_block2 Haddr_block2 "Hblock" "Hcode'".
+    cbn in Haddr_block2.
+    iMod (na_inv_acc with "HlinkInv Hna") as "(>Hassert_entry & Hna & Hclose)"; [ solve_ndisj.. |].
+    iApply assert_reg_success; last iFrame "#∗"; try solve_pure ; try reflexivity.
+    solve_ndisj.
+    iIntros "!> (HPC & Hr0 & Hr1 & Hr2 & Hr4 & Hr5 & Hblock & Hna & Hassert_entry)".
+    iMod ("Hclose" with "[$Hna $Hassert_entry]") as "Hna".
+    iAssert (codefrag addr_block2 pc_v' (assert_reg_instrs assert_lt_offset r_t1)) with "[$Hblock]" as "Hblock".
+    unfocus_block "Hblock" "Hcode'" as "Hcode".
+
+    focus_block 3%nat "Hcode" as addr_block3 Haddr_block3 "Hblock" "Hcode'".
+    iInstr "Hblock".
+    iInstr "Hblock".
+    iInstr "Hblock".
+    unfocus_block "Hblock" "Hcode'" as "Hcode".
+    replace (addr_block3 ^+ 2)%a with (a_data ^+ -2)%a by solve_addr'.
+
+    iApply (wp_wand with "[-]") ; [  | iIntros (?) "H"; iLeft ; iApply "H"].
+    iApply "Hcont"; iFrame.
+  Admitted.
+
+  Definition ts_main_inv b_main e_main pc_v main_code a_data link_cap ts_mainN
+    := na_inv logrel_nais ts_mainN
+         (codefrag b_main pc_v main_code
+          ∗ (a_data, pc_v) ↦ₐ link_cap
+          ∗ ((a_data ^+ 1)%a, pc_v) ↦ₐ LCap RWX b_main e_main a_data pc_v).
+
+  Lemma trusted_memory_readout_callback_code_sentry
+    (b_main : Addr) (pc_v : Version) (ts_mainN : namespace)
+
+    (b_link a_link e_link assert_entry : Addr) (link_tableN : namespace) (* linking *)
+    (assert_lt_offset : Z)
+    (b_assert e_assert a_flag : Addr) (v_assert : Version) (assertN flag_assertN : namespace) (* assert *)
+    :
+
+    let v_link := pc_v in
+    let link_cap := LCap RO b_link e_link a_link v_link in
+
+    let e_main := (b_main ^+ trusted_memory_readout_main_len)%a in
+    let a_callback := (b_main ^+ trusted_memory_readout_main_init_len)%a in
+    let a_data := (b_main ^+ trusted_memory_readout_main_code_len)%a in
+
+    let trusted_memory_readout_main := trusted_memory_readout_main_code assert_lt_offset in
+
+    assertN ## link_tableN ->
+    assertN ## ts_mainN ->
+    link_tableN ## ts_mainN ->
+    clientN ## ts_mainN ->
+    sensorN ## ts_mainN ->
+
+    ContiguousRegion b_main trusted_memory_readout_main_len ->
+    SubBounds b_main (b_main ^+ trusted_memory_readout_main_len)%a b_main
+      (b_main ^+ trusted_memory_readout_main_len)%a ->
+
+    (a_link + assert_lt_offset)%a = Some assert_entry →
+    withinBounds b_link e_link assert_entry = true ->
+    (link_table_inv
+       v_link
+       assert_entry b_assert e_assert v_assert link_tableN
+     ∗ assert_inv b_assert a_flag e_assert v_assert assertN
+     ∗ flag_inv a_flag v_assert flag_assertN
+     ∗ ts_main_inv b_main e_main pc_v (trusted_memory_readout_main_code assert_lt_offset) a_data link_cap ts_mainN
+    )
+    ∗ (system_inv (enclaves_map := contract_ts_enclaves_map))
+    ⊢ interp (LCap E b_main (b_main ^+ trusted_memory_readout_main_len)%a
+                (b_main ^+ trusted_memory_readout_main_init_len)%a pc_v).
+  Proof.
+    intros ??????????? HcontRegion HsubBounds Hassert Hlink.
+    iIntros "[#(HlinkInv & HassertInv & HflagInv & HcodeInv) #Hcemap_inv]".
+    iEval (rewrite fixpoint_interp1_eq /=).
+    iIntros (regs); iNext ; iModIntro.
+    iIntros "( [%Hrmap_full #Hrmap_interp] & Hrmap & Hna)".
+    rewrite /registers_mapsto.
+    iExtract "Hrmap" PC as "HPC".
+    cbn in Hrmap_full.
+    destruct (Hrmap_full r_t0) as [w0 Hr0].
+    destruct (Hrmap_full r_t1) as [w1 Hr1].
+    destruct (Hrmap_full r_t2) as [w2 Hr2].
+    destruct (Hrmap_full r_t3) as [w3 Hr3].
+    destruct (Hrmap_full r_t4) as [w4 Hr4].
+    destruct (Hrmap_full r_t5) as [w5 Hr5].
+    iExtractList "Hrmap" [r_t0;r_t1;r_t2;r_t3;r_t4;r_t5]
+      as ["Hr0";"Hr1";"Hr2";"Hr3";"Hr4";"Hr5"].
+
+    iAssert (interp w0) as "Hinterp_w0".
+    { iApply "Hrmap_interp";eauto;done. }
+    iAssert (interp w1) as "Hinterp_w1".
+    { iApply "Hrmap_interp";eauto;done. }
+
+    rewrite /interp_conf.
+    iApply (wp_wand _ _ _
+              ( fun v =>
+                  ((⌜v = HaltedV⌝ →
+                    ∃ lregs : LReg, full_map lregs
+                                    ∧ registers_mapsto lregs
+                                    ∗ na_own logrel_nais ⊤)
+                   ∨ ⌜v = FailedV⌝
+                  )%I)
+             with "[-]").
+
+    - iMod (na_inv_acc with "HcodeInv Hna") as "[>(Hcode & Hdata & Hdata') [Hna Hcls] ]"
+      ;[solve_ndisj|solve_ndisj|].
+
+      iApply ( (trusted_memory_readout_callback_code_spec (⊤ ∖ ↑ts_mainN))
+               with "[$HlinkInv $HassertInv $HflagInv $Hcemap_inv Hinterp_w0 Hinterp_w1]
+                 [$HPC $Hr0 $Hr1 $Hr2 $Hr3 $Hr4 $Hr5 $Hcode $Hdata $Hdata' $Hna Hcls Hrmap]")
+      ; eauto
+      ; eauto
+      ; try solve_ndisj
+      ; try iFrame "∗#".
+      iNext; iIntros "(Hcode & Hadata & Hadata' & HPC & Hr0 & Hr1 & Hr2 & Hr3 & Hr4 & Hr5 & Hna)".
+      iMod ("Hcls" with "[$Hcode $Hadata $Hadata' $Hna]") as "Hna".
+      wp_end. iIntros (_).
+      iDestruct (big_sepM_insert _ _ r_t5 with "[$Hrmap $Hr5]") as "Hrmap"
+      ; first (by rewrite lookup_delete).
+      rewrite insert_delete_insert; repeat (rewrite -delete_insert_ne //=).
+      iDestruct (big_sepM_insert _ _ r_t4 with "[$Hrmap $Hr4]") as "Hrmap"
+      ; first (by rewrite lookup_delete).
+      rewrite insert_delete_insert; repeat (rewrite -delete_insert_ne //=).
+      iDestruct (big_sepM_insert _ _ r_t3 with "[$Hrmap $Hr3]") as "Hrmap"
+      ; first (by rewrite lookup_delete).
+      rewrite insert_delete_insert; repeat (rewrite -delete_insert_ne //=).
+      iDestruct (big_sepM_insert _ _ r_t2 with "[$Hrmap $Hr2]") as "Hrmap"
+      ; first (by rewrite lookup_delete).
+      rewrite insert_delete_insert; repeat (rewrite -delete_insert_ne //=).
+      iDestruct (big_sepM_insert _ _ r_t1 with "[$Hrmap $Hr1]") as "Hrmap"
+      ; first (by rewrite lookup_delete).
+      rewrite insert_delete_insert; repeat (rewrite -delete_insert_ne //=).
+      iDestruct (big_sepM_insert _ _ r_t0 with "[$Hrmap $Hr0]") as "Hrmap"
+      ; first (by rewrite lookup_delete).
+      rewrite insert_delete_insert; repeat (rewrite -delete_insert_ne //=).
+      iDestruct (big_sepM_insert _ _ PC with "[$Hrmap $HPC]") as "Hrmap"
+      ; first (by rewrite lookup_delete).
+      rewrite insert_delete_insert; repeat (rewrite -delete_insert_ne //=).
+      iExists _.
+      iFrame "∗".
+
+
+      iPureIntro; intros r; cbn.
+      destruct (decide (r=PC)); simplify_map_eq;first done.
+      destruct (decide (r=r_t5)); simplify_map_eq;first done.
+      destruct (decide (r=r_t4)); simplify_map_eq;first done.
+      destruct (decide (r=r_t3)); simplify_map_eq;first done.
+      destruct (decide (r=r_t2)); simplify_map_eq;first done.
+      destruct (decide (r=r_t1)); simplify_map_eq;first done.
+      destruct (decide (r=r_t0)); simplify_map_eq;first done.
+      apply Hrmap_full.
+    - iEval (cbn). iIntros (v) "H ->".
+      iDestruct "H" as "[H|%]"; last congruence.
+      by iApply "H".
+  Qed.
+
+End trusted_memory_readout_main.
