theories/examples/enclaves/trusted_memory_readout_spec.v
@@ -1,0 +1,117 @@
+From iris.proofmode Require Import proofmode.
+From cap_machine Require Import rules logrel fundamental.
+From cap_machine Require Import proofmode.
+From cap_machine Require Import assert macros_new.
+From cap_machine Require Import
+  trusted_memory_readout_code
+  trusted_memory_readout_enclaves_spec
+  trusted_memory_readout_main_spec
+.
+
+Section trusted_memory_readout_full_run.
+  Context {Σ:gFunctors} {ceriseg:ceriseG Σ} {sealsg: sealStoreG Σ}
+    {oneshotg : one_shotG Σ} {nainv: logrel_na_invs Σ}
+    {reservedaddresses : ReservedAddresses}
+    `{MP: MachineParameters}.
+  Context {CS: ClientSensor}.
+
+  Lemma trusted_memory_readout_full_run_spec
+    (b_main : Addr) (pc_v : Version) (ts_mainN : namespace)
+
+    (b_link a_link e_link assert_entry : Addr) (link_tableN : namespace) (* linking *)
+    (assert_lt_offset : Z)
+    (b_assert e_assert a_flag : Addr) (v_assert : Version) (assertN flag_assertN : namespace) (* assert *)
+
+    (rmap : LReg)
+    (wadv : LWord)
+    :
+
+    let v_link := pc_v in
+    let link_cap := LCap RO b_link e_link a_link v_link in
+
+    let e_main := (b_main ^+ trusted_memory_readout_main_len)%a in
+    let a_callback := (b_main ^+ trusted_memory_readout_main_init_len)%a in
+    let a_data := (b_main ^+ trusted_memory_readout_main_code_len)%a in
+
+    let trusted_memory_readout_main := trusted_memory_readout_main_code assert_lt_offset in
+
+    assertN ## link_tableN ->
+    assertN ## ts_mainN ->
+    link_tableN ## ts_mainN ->
+    clientN ## ts_mainN ->
+    sensorN ## ts_mainN ->
+
+    ContiguousRegion b_main trusted_memory_readout_main_len ->
+    SubBounds b_main (b_main ^+ trusted_memory_readout_main_len)%a b_main
+      (b_main ^+ trusted_memory_readout_main_len)%a ->
+
+
+    (a_link + assert_lt_offset)%a = Some assert_entry →
+    withinBounds b_link e_link assert_entry = true ->
+
+    dom rmap = all_registers_s ∖ {[ PC; r_t0 ]} →
+
+    (link_table_inv
+       v_link
+       assert_entry b_assert e_assert v_assert link_tableN
+    ∗ assert_inv b_assert a_flag e_assert v_assert assertN
+    ∗ flag_inv a_flag v_assert flag_assertN
+    ∗ ts_main_inv b_main e_main pc_v (trusted_memory_readout_main_code assert_lt_offset) a_data link_cap ts_mainN
+    )
+    ∗ (system_inv (enclaves_map := contract_ts_enclaves_map))
+    ∗ interp wadv
+
+    ⊢ (PC ↦ᵣ LCap RWX b_main e_main b_main pc_v
+          ∗ r_t0 ↦ᵣ wadv
+          ∗ ([∗ map] r↦w ∈ rmap, r ↦ᵣ w ∗ ⌜is_zL w = true⌝)
+          ∗ na_own logrel_nais ⊤
+          -∗ WP Seq (Instr Executable) {{λ v,
+                  (⌜v = HaltedV⌝ → ∃ r : LReg, full_map r ∧ registers_mapsto r ∗ na_own logrel_nais ⊤)%I
+                  ∨ ⌜v = FailedV⌝ }})%I.
+  Proof.
+    intros ??????????? Hregion HsubBounds Hassert Hlink Hrmap.
+
+    iIntros "[  #(HlinkInv & HassertInv & HflagInv & HcodeInv) #[ Hcemap_inv Hinterp_wadv ] ]
+             (HPC & Hr0 & Hrmap & Hna)".
+
+    iDestruct (jmp_to_unknown wadv with "[] [$Hinterp_wadv]") as "Hjmp".
+    { iSplit; last iFrame "Hcemap_inv".
+      iModIntro.
+      iApply enclaves_contract.
+    }
+    iMod (na_inv_acc with "HcodeInv Hna") as "[>(Hcode & Hadata & Hadata') [Hna Hcls] ]"
+    ;[solve_ndisj|solve_ndisj|].
+
+    iExtract "Hrmap" r_t1 as "[Hr1 _]".
+    iApply (trusted_memory_readout_main_init_spec with "[-]"); eauto; iFrame.
+    iNext; iIntros "(Hcode & HPC & Hr0 & Hr1)".
+    iMod ("Hcls" with "[$Hcode $Hadata $Hadata' $Hna]") as "Hna".
+
+    set (rmap' := delete r_t1 rmap).
+    (* Show that the contents of unused registers is safe *)
+    iAssert ([∗ map] r↦w ∈ rmap', r ↦ᵣ w ∗ interp w)%I with "[Hrmap]" as "Hrmap".
+    { iApply (big_sepM_mono with "Hrmap"). intros r w Hr'. cbn.
+      iIntros "[Hr %Hw]". iFrame.
+      destruct_word w; try by inversion Hw. rewrite fixpoint_interp1_eq //.
+    }
+
+    (* Show the content of r1 is safe *)
+    iDestruct (trusted_memory_readout_callback_code_sentry
+                with "[$HlinkInv $HassertInv $HflagInv $HcodeInv $Hcemap_inv]")
+      as "Hinterp_wret"; eauto.
+    (* Cannot use iInsert, because Qed is too long *)
+    subst rmap'.
+    iDestruct (big_sepM_insert _ _ r_t1 with "[$Hrmap $Hr1 $Hinterp_wret]") as "Hrmap"
+    ; first (apply lookup_delete_None ; left ; done).
+    rewrite insert_delete_insert.
+    iDestruct (big_sepM_insert _ _ r_t0 with "[$Hrmap $Hr0 $Hinterp_wadv]") as "Hrmap"
+    ; first (rewrite lookup_insert_ne //=; apply not_elem_of_dom_1; rewrite Hrmap; set_solver).
+
+    (* Apply the result of the FTLR *)
+    iApply (wp_wand with "[-]").
+    - iApply ("Hjmp" with "[] [$HPC $Hrmap $Hna]") ;eauto.
+      iPureIntro; rewrite !dom_insert_L Hrmap; set_solver.
+    - iIntros (v) "H"; by iLeft.
+  Qed.
+
+End trusted_memory_readout_full_run.
